Progress on bridging lemma.

common/UCComposition.ec
@@ -118,7 +118,7 @@ module MakeRFComp (Rest : FUNC, Par : FUNC) : FUNC = {
 clone MakeInterface as MakeInt'
 proof *.
 
-module MI' = MakeInt.MI.
+module MI' = MakeInt'.MI.
 
 module CompEnv (Rest : FUNC, Env : ENV, Inter : INTER) = {
   var stub_st : msg option
@@ -201,10 +201,10 @@ op rest_adv_pi_ok (guard : int fset) : bool =
 
 section.
 
-declare module Env  <: ENV.
-declare module Adv  <: ADV{-Env}.
-declare module Rest <: FUNC{-Env, -Adv}.
-declare module Par  <: FUNC{-Env, -Adv, -Rest}.
+declare module Env  <: ENV{-MI, -CompEnv}.
+declare module Adv  <: ADV{-MI, -CompEnv, -Env}.
+declare module Rest <: FUNC{-MI, -CompEnv, -Env, -Adv}.
+declare module Par  <: FUNC{-MI, -CompEnv, -Env, -Adv, -Rest}.
 
 declare op invar_rest : glob Rest -> bool.
 declare op term_rest  : glob Rest -> int.
@@ -215,13 +215,13 @@ declare op term_par   : glob Par  -> int.
 declare axiom ge0_term_rest (gl : glob Rest) :
   0 <= term_rest gl.
 
-declare axiom rest_init :
+declare axiom Rest_init :
    equiv
    [Rest.init ~ Rest.init :
     ={self} ==>
     ={glob Rest} /\ invar_rest (glob Rest){1}].
 
-declare axiom rest_invoke (n : int) :
+declare axiom Rest_invoke (n : int) :
    equiv
    [Rest.invoke ~ Rest.invoke :
     ={m, glob Rest} /\ invar_rest (glob Rest){1} /\
@@ -232,13 +232,13 @@ declare axiom rest_invoke (n : int) :
 declare axiom ge0_term_par (gl : glob Par) :
   0 <= term_par gl.
 
-declare axiom par_init :
+declare axiom Par_init :
    equiv
    [Par.init ~ Par.init :
     ={self} ==>
     ={glob Par} /\ invar_par (glob Par){1}].
 
-declare axiom par_invoke (n : int) :
+declare axiom Par_invoke (n : int) :
    equiv
    [Par.invoke ~ Par.invoke :
     ={m, glob Par} /\ invar_par (glob Par){1} /\
@@ -257,15 +257,57 @@ lemma comp_bridge
   Pr[Exper(MI(Par, Adv), CompEnv(Rest, Env))
        .main(func' ++ [change_pari], in_guard_hi') @ &m : res].
 proof.
+move =>
+  ep_func' sub_in_guard_low'_in_guard_high' rest_adv_pi_ok_in_guard_hi'
+  eq_in_guard_low_ce_in_guard_low'.
+byequiv => //.
+proc; inline *; wp.
+swap{2} 6 14; swap{2} 5 14; swap{2} 17 1; sp.
+seq 3 3 :
+  (={glob Env, glob Adv, glob Rest, glob Par} /\
+   invar_rest (glob Rest){1} /\ invar_par (glob Par){1} /\
+   _self{1} = func' /\ _self{1} = func{1} /\
+   _self{1} = MI.func{1} /\ _self{1} = MakeRFComp.self{1} /\
+   in_guard{1} = in_guard_low' /\ in_guard{1} = MI.in_guard{1} /\
+   _self{2} = func' /\ _self{2} = func0{2} /\ _self{2} = MI'.func{2} /\
+   _self{2} = MakeRFComp.self{2} /\ _self{2} = CompEnv.func{2} /\
+   MI.func{2} = func' ++ [change_pari] /\
+   in_guard1{2} = CompEnv.in_guard_low{2} /\
+   in_guard1{2} = MI'.in_guard{2} /\
+   in_guard1{2} = in_guard_low' /\
+   MI.in_guard{2} = in_guard_hi' /\
+   CompEnv.stub_st{2} = None).
+call (_ : true).
+call Par_init.
+call Rest_init.
+auto; progress;
+  by rewrite size_cat /= take_size_cat.
+call
+  (_ :
+   ={glob Adv, glob Rest, glob Par} /\
+   invar_rest (glob Rest){1} /\ invar_par (glob Par){1} /\
+   MI.func{1} = func' /\ MakeRFComp.self{1} = func' /\
+   MI.in_guard{1} = in_guard_low' /\
+   MI'.func{2} = func' /\ MakeRFComp.self{2} = func' /\
+   CompEnv.func{2} = func' /\ MI.func{2} = func' ++ [change_pari] /\
+   CompEnv.in_guard_low{2} = in_guard_low' /\
+   MI'.in_guard{2} = in_guard_low' /\ MI.in_guard{2} = in_guard_hi' /\
+   CompEnv.stub_st{2} = None).
+proc.
+if => //.
+inline loop.
+sp 3 3.
 admit.
+auto.
+auto.
 qed.
 
 end section.
 
 lemma compos_bridge
-      (Env <: ENV) (Adv <: ADV{-Env})
-      (Rest <: FUNC{-Env, -Adv})
-      (Par <: FUNC{-Env, -Adv, -Rest})
+      (Env <: ENV{-MI, -CompEnv}) (Adv <: ADV{-MI, -CompEnv, -Env})
+      (Rest <: FUNC{-MI, -CompEnv, -Env, -Adv})
+      (Par <: FUNC{-MI, -CompEnv, -Env, -Adv, -Rest})
       (invar_rest : glob Rest -> bool, term_rest : glob Rest -> int,
        invar_par : glob Par -> bool, term_par : glob Par -> int)
       (func' : addr, in_guard_low' in_guard_hi' : int fset) &m :
